proof/crefine/RISCV64/Interrupt_C.thy
@@ -92,7 +92,7 @@ proof -
                     ghost_assertion_data_set_def)
   apply (clarsimp simp: cte_at_irq_node' ucast_nat_def)
   apply (clarsimp simp: cte_wp_at_ctes_of badge_derived'_def
-                        Collect_const_mem unat_gt_0 valid_cap_simps' RISCV64.maxIRQ_def)
+                        Collect_const_mem unat_gt_0 valid_cap_simps' maxIRQ_def)
   apply (drule word_le_nat_alt[THEN iffD1])
   apply clarsimp
   apply (drule valid_globals_ex_cte_cap_irq[where irq=irq])
@@ -276,7 +276,7 @@ lemma decodeIRQHandlerInvocation_ccorres:
      apply (auto dest: st_tcb_at_idle_thread' ctes_of_valid')[6]
     apply (drule ctes_of_valid')
      apply fastforce
-    apply (clarsimp simp add:valid_cap_simps' RISCV64.maxIRQ_def)
+    apply (clarsimp simp add:valid_cap_simps' maxIRQ_def)
     apply (erule order.trans,simp)
   apply (auto dest: st_tcb_at_idle_thread' ctes_of_valid')
   done
@@ -367,8 +367,8 @@ lemma isIRQActive_ccorres:
   done
 
 lemma Platform_maxIRQ:
-  "RISCV64.maxIRQ = scast Kernel_C.maxIRQ"
-   by (simp add: RISCV64.maxIRQ_def Kernel_C.maxIRQ_def)
+  "maxIRQ = scast Kernel_C.maxIRQ"
+   by (simp add: maxIRQ_def Kernel_C.maxIRQ_def)
 
 lemma Arch_invokeIRQControl_ccorres:
   "ccorres (K (K \<bottom>) \<currency> dc) (liftxf errstate id (K ()) ret__unsigned_long_')
